sepcomp/backend/Renumberproof_sepcomp.v
@@ -196,22 +196,6 @@ Inductive match_frames: RTL.stackframe -> RTL.stackframe -> Prop :=
       match_frames (Stackframe res f sp pc rs)
                    (Stackframe res f sp pc rs).
 
-Inductive match_transl_states: RTL.state -> RTL.state -> Prop :=
-| match_transl_regular_states: forall stk f sp pc rs m stk'
-        (STACKS: list_forall2 match_frames stk stk')
-        (REACH: reach f pc),
-      match_transl_states (State stk f sp pc rs m)
-                   (State stk' (transf_function f) sp (renum_pc (pnum f) pc) rs m)
-| match_transl_callstates: forall stk f f' args m stk'
-        (FD: match_fundef f f')
-        (STACKS: list_forall2 match_frames stk stk'),
-      match_transl_states (Callstate stk f args m)
-                   (Callstate stk' f' args m)
-| match_transl_returnstates: forall stk v m stk'
-        (STACKS: list_forall2 match_frames stk stk'),
-      match_transl_states (Returnstate stk v m)
-                   (Returnstate stk' v m).
-
 Inductive match_identical_states: RTL.state -> RTL.state -> Prop :=
 | match_identical_regular_states: forall stk f sp pc rs m stk'
         (STACKS: list_forall2 match_frames stk stk'),
@@ -219,108 +203,22 @@ Inductive match_identical_states: RTL.state -> RTL.state -> Prop :=
                    (State stk' f sp pc rs m).
 
 Inductive match_states: RTL.state -> RTL.state -> Prop :=
-| match_states_transl: forall st1 st2
-                              (MSTATE: match_transl_states st1 st2),
-                         match_states st1 st2
-| match_states_identical: forall st1 st2
-                              (MSTATE: match_identical_states st1 st2),
-                         match_states st1 st2.
-
-Lemma step_simulation_transl:
-  forall S1 t S2, RTL.step ge S1 t S2 ->
-  forall S1', match_transl_states S1 S1' ->
-  exists S2', RTL.step tge S1' t S2' /\ match_states S2 S2'.
-Proof.
-  induction 1; intros S1' MS; inv MS; try TR_AT.
-(* nop *)
-  econstructor; split. eapply exec_Inop; eauto. 
-  constructor; auto. constructor; eauto. eapply reach_succ; eauto. simpl; auto. 
-(* op *)
-  econstructor; split.
-  eapply exec_Iop; eauto.
-  instantiate (1 := v). rewrite <- H0. apply eval_operation_preserved. exact symbols_preserved. 
-  constructor; auto. constructor; auto. eapply reach_succ; eauto. simpl; auto.
-(* load *)
-  econstructor; split.
-  assert (eval_addressing tge sp addr rs ## args = Some a).
-  rewrite <- H0. apply eval_addressing_preserved. exact symbols_preserved. 
-  eapply exec_Iload; eauto.
-  constructor; auto. constructor; auto. eapply reach_succ; eauto. simpl; auto.
-(* store *)
-  econstructor; split.
-  assert (eval_addressing tge sp addr rs ## args = Some a).
-  rewrite <- H0. apply eval_addressing_preserved. exact symbols_preserved. 
-  eapply exec_Istore; eauto.
-  constructor; auto. constructor; auto. eapply reach_succ; eauto. simpl; auto.
-(* call *)
-  exploit find_function_translated; eauto.
-  intros Htfd. destruct Htfd as [tfd [findtfd matchtfd]].
-  econstructor; split.
-  eapply exec_Icall with (fd := tfd); eauto.
-  inv matchtfd; auto.
-    apply sig_preserved.
-  constructor; auto. constructor; auto. constructor; auto. constructor; auto. eapply reach_succ; eauto. simpl; auto.
-(* tailcall *)
-  exploit find_function_translated; eauto.
-  intros Htfd. destruct Htfd as [tfd [findtfd matchtfd]].
-  econstructor; split.
-  eapply exec_Itailcall with (fd := tfd); eauto.
-  inv matchtfd; auto.
-    apply sig_preserved.
-  constructor. auto.
-  constructor; auto.
-(* builtin *)
-  econstructor; split.
-  eapply exec_Ibuiltin; eauto.
-    eapply external_call_symbols_preserved; eauto.
-    exact symbols_preserved. exact varinfo_preserved.
-  constructor; auto. constructor; auto. eapply reach_succ; eauto. simpl; auto.
-(* cond *)
-  econstructor; split.
-  eapply exec_Icond; eauto. 
-  replace (if b then renum_pc (pnum f) ifso else renum_pc (pnum f) ifnot)
-     with (renum_pc (pnum f) (if b then ifso else ifnot)).
-  constructor; auto. constructor; auto. eapply reach_succ; eauto. simpl. destruct b; auto. 
-  destruct b; auto.
-(* jumptbl *)
-  econstructor; split.
-  eapply exec_Ijumptable; eauto. rewrite list_nth_z_map. rewrite H1. simpl; eauto. 
-  constructor; auto. constructor; auto. eapply reach_succ; eauto. simpl. eapply list_nth_z_in; eauto. 
-(* return *)
-  econstructor; split.
-  eapply exec_Ireturn; eauto. 
-  constructor.
-  constructor; auto.
-(* internal function *)
-  inv FD.
-  (* call translated *)
-  simpl. econstructor; split.
-  eapply exec_function_internal; eauto. 
-  constructor. constructor; auto. unfold reach. constructor.
-  (* call identical *)
-  simpl. econstructor; split.
-  eapply exec_function_internal; eauto.
-  apply match_states_identical. constructor; auto.
-(* external function *)
-  assert (f' = AST.External ef); subst.
-  { inv FD; auto. }
-  econstructor; split.
-  eapply exec_function_external; eauto.
-    eapply external_call_symbols_preserved; eauto.
-    exact symbols_preserved. exact varinfo_preserved.
-  constructor. constructor; auto.
-(* return *)
-  inv STACKS. inv H1.
-  (* transl *)
-  econstructor; split. 
-  eapply exec_return; eauto. 
-  constructor. constructor; auto.
-  (* identical *)
-  econstructor; split. 
-  eapply exec_return; eauto.
-  apply match_states_identical.
-  constructor; auto.
-Qed.
+| match_regular_states: forall stk f sp pc rs m stk'
+        (STACKS: list_forall2 match_frames stk stk')
+        (REACH: reach f pc),
+      match_states (State stk f sp pc rs m)
+                   (State stk' (transf_function f) sp (renum_pc (pnum f) pc) rs m)
+| match_callstates: forall stk f f' args m stk'
+        (FD: match_fundef f f')
+        (STACKS: list_forall2 match_frames stk stk'),
+      match_states (Callstate stk f args m)
+                   (Callstate stk' f' args m)
+| match_returnstates: forall stk v m stk'
+        (STACKS: list_forall2 match_frames stk stk'),
+      match_states (Returnstate stk v m)
+                   (Returnstate stk' v m)
+| match_states_identical: forall s s' (MATCH: match_identical_states s s'),
+                            match_states s s'.
 
 Lemma step_simulation_identical:
   forall S1 t S2, RTL.step ge S1 t S2 ->
@@ -332,12 +230,9 @@ Proof.
     destruct S1; try by inv NORMAL1.
     exploit is_normal_step; eauto. intro. des. subst.
     inv MS.
-    exploit is_normal_identical;
-      try apply symbols_preserved;
-      try apply varinfo_preserved;
-      eauto.
+    exploit is_normal_identical; eauto using symbols_preserved, varinfo_preserved.
     intro. des.
-    eexists. split. eauto.
+    eexists. split;eauto.
     apply match_states_identical. econs; eauto.
   }
   inv MS. unfold is_normal in NORMAL1.
@@ -346,13 +241,9 @@ Proof.
     inv H; clarify.
     exploit find_function_translated; eauto.
     intro. des.
-    eexists. split.
-    { eapply exec_Icall; eauto.
-      eapply match_fundef_sig. eauto.
-    }
-    econs. econs; eauto.
-    constructor; eauto.
-    eapply match_frames_identical; eauto.
+    eexists. split; eauto using exec_Icall, match_fundef_sig.
+    econs; eauto.
+    constructor; eauto using match_frames_identical.
   - (* Itailcall *)
     inv H; clarify.
     exploit find_function_translated; eauto.
@@ -361,24 +252,111 @@ Proof.
     { eapply exec_Itailcall; eauto.
       eapply match_fundef_sig. eauto.
     }
-    econs. econs; eauto.
+    econs; eauto.
   - (* Ireturn *)
     inv H; clarify.
     eexists. split.
     { eapply exec_Ireturn; eauto. }
-    econs. econs; eauto.
+    econs; eauto.
 Qed.
 
 Lemma step_simulation:
   forall S1 t S2, RTL.step ge S1 t S2 ->
-  forall S1' (MS: match_states S1 S1'),
+  forall S1', match_states S1 S1' ->
   exists S2', RTL.step tge S1' t S2' /\ match_states S2 S2'.
 Proof.
-  intros. inv MS.
-  - eapply step_simulation_transl; eauto.
-  - eapply step_simulation_identical; eauto.
+  intros s1 t s2 BACKUP_STEP. generalize BACKUP_STEP.
+
+  induction 1; intros S1' MS; inv MS;
+  try (by eauto using step_simulation_identical); try TR_AT.
+
+(* nop *)
+  econstructor; split. eapply exec_Inop; eauto. 
+  constructor; auto. eapply reach_succ; eauto. simpl; auto. 
+(* op *)
+  econstructor; split.
+  eapply exec_Iop; eauto.
+  instantiate (1 := v). rewrite <- H0. apply eval_operation_preserved. exact symbols_preserved. 
+  constructor; auto. eapply reach_succ; eauto. simpl; auto.
+(* load *)
+  econstructor; split.
+  assert (eval_addressing tge sp addr rs ## args = Some a).
+  rewrite <- H0. apply eval_addressing_preserved. exact symbols_preserved. 
+  eapply exec_Iload; eauto.
+  constructor; auto. eapply reach_succ; eauto. simpl; auto.
+(* store *)
+  econstructor; split.
+  assert (eval_addressing tge sp addr rs ## args = Some a).
+  rewrite <- H0. apply eval_addressing_preserved. exact symbols_preserved. 
+  eapply exec_Istore; eauto.
+  constructor; auto. eapply reach_succ; eauto. simpl; auto.
+(* call *)
+  exploit find_function_translated; eauto.
+  intros Htfd. destruct Htfd as [tfd [findtfd matchtfd]].
+  econstructor; split.
+  eapply exec_Icall with (fd := tfd); eauto.
+  inv matchtfd; auto.
+    apply sig_preserved.
+  constructor; auto. constructor; auto. constructor; auto. eapply reach_succ; eauto. simpl; auto.
+(* tailcall *)
+  exploit find_function_translated; eauto.
+  intros Htfd. destruct Htfd as [tfd [findtfd matchtfd]].
+  econstructor; split.
+  eapply exec_Itailcall with (fd := tfd); eauto.
+  inv matchtfd; auto.
+    apply sig_preserved.
+  constructor; auto.
+(* builtin *)
+  econstructor; split.
+  eapply exec_Ibuiltin; eauto.
+    eapply external_call_symbols_preserved; eauto.
+    exact symbols_preserved. exact varinfo_preserved.
+  constructor; auto. eapply reach_succ; eauto. simpl; auto.
+(* cond *)
+  econstructor; split.
+  eapply exec_Icond; eauto. 
+  replace (if b then renum_pc (pnum f) ifso else renum_pc (pnum f) ifnot)
+     with (renum_pc (pnum f) (if b then ifso else ifnot)).
+  constructor; auto. eapply reach_succ; eauto. simpl. destruct b; auto. 
+  destruct b; auto.
+(* jumptbl *)
+  econstructor; split.
+  eapply exec_Ijumptable; eauto. rewrite list_nth_z_map. rewrite H1. simpl; eauto. 
+  constructor; auto. eapply reach_succ; eauto. simpl. eapply list_nth_z_in; eauto. 
+(* return *)
+  econstructor; split.
+  eapply exec_Ireturn; eauto. 
+  constructor; auto.
+(* internal function *)
+  inv FD.
+  (* call translated *)
+  simpl. econstructor; split.
+  eapply exec_function_internal; eauto. 
+  constructor; auto. unfold reach. constructor.
+  (* call identical *)
+  simpl. econstructor; split.
+  eapply exec_function_internal; eauto.
+  apply match_states_identical. constructor; auto.
+(* external function *)
+  assert (f' = AST.External ef); subst.
+  { inv FD; auto. }
+  econstructor; split.
+  eapply exec_function_external; eauto.
+    eapply external_call_symbols_preserved; eauto.
+    exact symbols_preserved. exact varinfo_preserved.
+  constructor; auto.
+(* return *)
+  inv STACKS. inv H1.
+  (* transl *)
+  econstructor; split. 
+  eapply exec_return; eauto. 
+  constructor; auto.
+  (* identical *)
+  econstructor; split. 
+  eapply exec_return; eauto.
+  apply match_states_identical.
+  constructor; auto.
 Qed.
-  
 
 Lemma transf_initial_states:
   forall S1, RTL.initial_state prog S1 ->
@@ -396,13 +374,14 @@ Proof.
     eauto.    
     inv matchtf; auto.
     rewrite <- H3; apply sig_preserved.
-  constructor; auto. constructor; auto. constructor.
+  constructor; auto. constructor.
 Qed.
 
 Lemma transf_final_states:
   forall S1 S2 r, match_states S1 S2 -> RTL.final_state S1 r -> RTL.final_state S2 r.
 Proof.
-  intros. inv H0. inv H; inv MSTATE. inv STACKS. constructor.
+  intros. inv H0. inv H. inv STACKS. constructor.
+  inv MATCH.
 Qed.
 
 Theorem transf_program_correct:
